text/guide-level-explanation-example-2.dfy
@@ -1,18 +1,46 @@
 datatype Option<T> = Some(value: T) | None
 
+//
+// Wrapper around a concurrent data structure, such as
+// ConcurrentHashMap<K, V> in Java.
+//
+// Note the lack of a ghost variable to track the state of the map,
+// which intentionally puts the mutable state outside of the Dafny-verified model.
+// These methods instead appear to have non-deterministic behavior to Dafny, which accurately
+// represents the fact that it cannot assume anything about state that might be changed by
+// other threads.
+//
 class {:extern} ExternalMutableMap<K, V> {
-  method {:extern} Put(k: K, v: V)
-  method {:extern} Get(k: V) returns (v: Option<V>)
+  constructor {:extern} () reads {}
+  method {:extern} Put(k: K, v: V) reads {}
+  method {:extern} Get(k: V) returns (v: Option<V>) reads {}
 }
 
-method {:extern} SafeMemoizedFibonacci(n: int, cache: ExternalMutableMap<nat, nat>) returns (r: nat)
+class FibonacciMemoizer {
+  const cache: ExternalMutableMap<nat, nat>
+  constructor() reads {} {
+    cache := new ExternalMutableMap();
+  }
+  method Get(n: nat) returns (r: nat)
+    reads {}
+  {
+    if n <= 2 {
+      return 1;
+    }
+    var cached := cache.Get(n);
+    if cached.Some? {
+      r := cached.value;
+    } else {
+      var oneBefore := Get(n - 1);
+      var twoBefore := Get(n - 2);
+      r := oneBefore + twoBefore;
+      cache.Put(n, r);
+    }
+  }
+}
+
+method {:extern} SafeFibonacci(n: nat, memoizer: FibonacciMemoizer) returns (r: nat)
   reads {}
 {
-  var cached := cache.Get(n);
-  if cached.Some? {
-    r := cached.value;
-  } else {
-    r := Fibonacci(n);
-    cache.Put(n, r);
-  }
+  r := memoizer.Get(n);
 }
